io/RunningExample.fst
@@ -18,7 +18,7 @@ let did_not_respond h =
   | EWrite _ _ _ :: _ -> false
   | _ -> true
 
-val handler_only_openfiles_reads_client_acc : trace -> list file_descr -> bool
+val handler_only_openfiles_reads_client_acc : trace -> list file_descr -> Type0
 let rec handler_only_openfiles_reads_client_acc lt open_descrs =
   match lt with
   | [] -> true
@@ -40,7 +40,7 @@ let rec handler_only_openfiles_reads_client_acc lt open_descrs =
     if fd `mem` open_descrs then handler_only_openfiles_reads_client_acc tl (filter (fun fd' -> fd <> fd') open_descrs)
     else false
 
-val handler_only_openfiles_reads_client : trace -> bool
+val handler_only_openfiles_reads_client : trace -> Type0
 let handler_only_openfiles_reads_client lt =
   handler_only_openfiles_reads_client_acc lt []
 
@@ -52,19 +52,19 @@ let rec wrote_at_least_once_to client lt =
                          client = fd
   | _ :: tl -> wrote_at_least_once_to client tl 
 
-type request_handler =
+type request_handler (fl:erased tflag) =
   (client:file_descr) ->
   (req:string) ->
-  (send:(msg:string -> IIO (resexn unit) IOActions (requires (fun h -> valid_http_response msg /\
-                                                                      did_not_respond h))
-                                                   (ensures (fun _ _ lt -> exists r. lt == [EWrite true (client,msg) r] /\
+  (send:(msg:string -> IIO (resexn unit) fl (requires (fun h -> valid_http_response msg /\
+                                                               did_not_respond h))
+                                            (ensures (fun _ _ lt -> exists r. lt == [EWrite true (client,msg) r] /\
                                                                          wrote_at_least_once_to client lt)))) ->
-  IIO (resexn unit) IOActions (requires (fun h -> valid_http_request req /\ did_not_respond h))
-                              (ensures (fun h _ lt -> handler_only_openfiles_reads_client lt /\
-                                                    wrote_at_least_once_to client lt))
+  IIO (resexn unit) fl (requires (fun h -> valid_http_request req /\ did_not_respond h))
+                       (ensures (fun h r lt -> handler_only_openfiles_reads_client lt /\
+                                             (wrote_at_least_once_to client lt \/ Inr? r)))
 
 (** ** E.g. of source handler **)
-val source_handler : request_handler
+val source_handler : request_handler IOActions
 let source_handler client req send =
   let res = req_res req in
   let _ = send res in 
@@ -116,18 +116,18 @@ val every_request_gets_a_response : trace -> Type0
 let every_request_gets_a_response lt =
   every_request_gets_a_response_acc lt []
 
-assume val get_req : file_descr -> option (req:string{valid_http_request req})
+assume val get_req : file_descr -> (req:string{valid_http_request req})
 assume val sendError : int -> fd:file_descr -> IIO unit IOActions
  (fun _ -> True) (fun _ _ lt -> exists (msg:string) r. lt == [EWrite true (fd, msg) r])
 
 open FStar.Tactics
 (* This may take a bit of effort to prove. *)
-let webserver (handler:request_handler) :
-  IIO (resexn unit) IOActions
+let webserver (handler:request_handler IOActions) :
+  IIO int IOActions
     (requires (fun h -> True))
     (ensures (fun _ _ lt -> 
       every_request_gets_a_response lt))
-    by (
+(**    by (
       explode ();
       bump_nth 49; 
       l_to_r [`FStar.List.Tot.Properties.append_nil_l];
@@ -138,13 +138,15 @@ let webserver (handler:request_handler) :
         l_to_r [`FStar.List.Tot.Properties.append_nil_l];
       trefl ();
       tadmit ();
-      dump "H") =
+      dump "H")**) =
+  admit ();
   let client = static_cmd true Openfile "test.txt" in
-  match client with | Inr err -> Inr err | Inl client -> begin
-    match get_req client with
-    | Some req -> handler client req (fun res -> static_cmd true Write (client,res))
-    | None -> sendError 400 client;
-    static_cmd true Close client
+  match client with | Inr _ -> (-1) | Inl client -> begin
+  let req = get_req client in
+  (match handler client req (fun res -> static_cmd true Write (client,res)) with 
+  | Inr err -> sendError 400 client 
+  | Inl client -> ());
+  0
   end
 
 (** ** Instante source interface with the example **)
@@ -169,10 +171,34 @@ let pi h isTrusted cmd arg =
   | true, Write -> true
   | _ -> false
 
+val phi : enforced_policy pi
+let phi h cmd arg =
+  match cmd with
+  | Openfile -> 
+    if arg = "/temp" then true else false
+  | Read -> is_opened_by_untrusted h arg
+  | Close -> is_opened_by_untrusted h arg
+  | Write -> false
+
+let psi : trace -> int -> trace -> Type0 =
+  (fun _ _ lt -> every_request_gets_a_response lt)
+
 let rec lemma1 (lt h:trace) : Lemma (requires (enforced_locally pi h lt)) (ensures (handler_only_openfiles_reads_client lt)) =
   match lt with
   | [] -> ()
   | e::tl -> admit ()//  lemma1 tl (e::h)
 
+  (*
+let ct_rcs' : tree pck_rc = 
+  Node 
+    (| string, resexn unit, (fun msg h _ _ -> valid_http_response msg && did_not_respond h) |)
+    Leaf
+    Leaf
 
+
+let ct_rcs : tree pck_rc =
+  Node (| file_descr -> string -> trace -> resexn unit -> trace -> bool, (fun (client, req) _ _ lt -> wrote_at_least_once_to client lt) |)
+    ct_rcs'
+    Leaf
+*)
 (** ** Tests: compile web-server, back-translate handler, linking **)
